add benchmark of insert_avl
is_balanced currently not optimized
access to height in O(1) will be added
current theoretical complexity: O(n),
where n is the size of the tree
current measured  complexity: O(n)

test.c
@@ -1,13 +1,27 @@
 #include "P1_UInt32.c"
 
-int main() {
+int main(int argc, char** argv) {
+  if (argc == 1) {
+    puts("Please supply an argument.");
+    return 1;
+  }
+  if (argc > 2) {
+    puts("Please supply less arguments.");
+    return 2;
+  }
+  printf("%s\n", argv[0]);
   //uint32_t p = P1_UInt32_main ();
   //printf("r=%ui\n", p);
   //uint64_t h = P1_UInt32_main2 ();
   //printf("h=%lui\n", h);
   //uint64_t s = P1_UInt32_main3 ();
   //printf("s=%lui\n", s);
-  uint64_t r = P1_UInt32_main4 ();
-  printf("r=%lui\n", r);
+  //uint64_t r = P1_UInt32_main4 ();
+  //printf("r=%lui\n", r);
+  uint64_t x = strtoull(argv[1], NULL, 0);
+  uint64_t s = 0;
+  void* ptr = P1_UInt32_main5(x);
+  s = P1_UInt32_sot_wds(ptr);
+  printf("s=%lui\n", s);
   return 0;
 }
