P1_UInt32.fst
@@ -13,33 +13,41 @@ module I64 = FStar.Int64
 let t = Impl.Core.t
 let linked_tree = Impl.Core.linked_tree
 
-//let a = U32.t
-//let val0 = 0ul
-//let val1 = 1ul
-//let val2 = 2ul
-//let val3 = 3ul
-//let val4 = 4ul
-//let val42 = 42ul
-//let compare (x y: U32.t) : I64.t
+
+
+let a = U64.t
+
+//inline_for_extraction noextract
+let one = Impl.Common.one
+//inline_for_extraction noextract
+let zero = Impl.Common.zero
+
+let val0 = 0UL
+let val1 = 1UL
+let val2 = 2UL
+let val3 = 3UL
+let val4 = 4UL
+let val42 = 42UL
+let compare (x y: U64.t) : I64.t
+  =
+  if U64.gt x y then 1L
+  else if U64.eq x y then 0L
+  else -1L
+
+//let a = (U32.t & U32.t)
+//let val0 = 0ul, 0ul
+//let val1 = 1ul, 1ul
+//let val2 = 2ul, 2ul
+//let val3 = 3ul, 3ul
+//let val4 = 4ul, 4ul
+//let val42 = 42ul, 42ul
+//let compare (x y: a) : I64.t
 //  =
+//  let x = fst x in
+//  let y = fst y in
 //  if U32.gt x y then 1L
 //  else if U32.eq x y then 0L
 //  else -1L
-
-let a = (U32.t & U32.t)
-let val0 = 0ul, 0ul
-let val1 = 1ul, 1ul
-let val2 = 2ul, 2ul
-let val3 = 3ul, 3ul
-let val4 = 4ul, 4ul
-let val42 = 42ul, 42ul
-let compare (x y: a) : I64.t
-  =
-  let x = fst x in
-  let y = fst y in
-  if U32.gt x y then 1L
-  else if U32.eq x y then 0L
-  else -1L
 
 inline_for_extraction noextract
 let get_left = Impl.Core.get_left #a
@@ -182,22 +190,57 @@ let compare_is_cmp () : Lemma
 //  destruct ptr;
 //  return (fst vr)
 
-let main4()
-  : Steel U32.t
-  emp (fun _ -> emp)
+//let main4()
+//  : Steel U32.t
+//  emp (fun _ -> emp)
+//  (requires fun _ -> True)
+//  (ensures fun _ _ _ -> True)
+//  =
+//  let ptr = create_tree val3 in
+//  let valn1 = 2ul, 1729ul in
+//  let valn2 = 2ul, 42ul in
+//  // toggling this flag allow one to check
+//  // whether the r arg of insert_bst2 is taken into account
+//  let f = true in
+//  let ptr = insert_avl2 f compare ptr valn1 in
+//  let ptr = insert_avl2 f compare ptr valn2 in
+//  assert (I64.eq (compare valn1 valn2) I64.zero);
+//  let b = member compare ptr valn2 in
+//  let vr = if b then val42 else val0 in
+//  destruct ptr;
+//  return (fst vr)
+
+let rec main5_aux (ptr: t a) (v: a)
+  : Steel (t a)
+  (linked_tree ptr) (fun ptr' -> linked_tree ptr')
+  (requires fun h0 ->
+    True
+    //Spec.size_of_tree (v_linked_tree ptr h0) < 100
+  )
+  (ensures fun h0 ptr' h1 ->
+    //Spec.size_of_tree (v_linked_tree ptr h1)
+    //==
+    //Spec.size_of_tree (v_linked_tree ptr h0) + 1/\
+    //Spec.size_of_tree (v_linked_tree ptr h0) < 100
+    True
+  )
+  =
+  sladmit ();
+  if U64.eq v zero then (
+    let h = get () in
+    return ptr
+  ) else (
+    let ptr' = insert_avl2 true compare ptr v in
+    let v' = U64.sub v one in
+    main5_aux ptr' v'
+  )
+
+
+let main5 (x: a)
+  : Steel (t a)
+  emp (fun ptr -> linked_tree ptr)
   (requires fun _ -> True)
   (ensures fun _ _ _ -> True)
   =
-  let ptr = create_tree val3 in
-  let valn1 = 2ul, 1729ul in
-  let valn2 = 2ul, 42ul in
-  // toggling this flag allow one to check
-  // whether the r arg of insert_bst2 is taken into account
-  let f = true in
-  let ptr = insert_avl2 f compare ptr valn1 in
-  let ptr = insert_avl2 f compare ptr valn2 in
-  assert (I64.eq (compare valn1 valn2) I64.zero);
-  let b = member compare ptr valn2 in
-  let vr = if b then val42 else val0 in
-  destruct ptr;
-  return (fst vr)
+  let ptr = create_leaf () in
+  main5_aux ptr x
